middle

NuLLReps.thy
@@ -16,7 +16,7 @@ section \<open>Miscellaneous built-in\<close>
 instantiation void :: naive_lrep begin
 definition share_void :: "zint \<Rightarrow> void \<Rightarrow> void" where [simp]: "share_void z = id"
 definition shareable_void :: "void set" where [simp]: "shareable_void = UNIV"
-definition revert_void :: "void \<times> void \<Rightarrow> bool" where [simp]: "revert_void xy = True"
+definition revert_void :: "void \<Rightarrow> void \<Rightarrow> bool" where [simp]: "revert_void x y = True"
 definition dpriv_void :: "void \<Rightarrow> void" where [simp]: "dpriv_void x = x"
 instance by standard auto
 end
@@ -31,7 +31,7 @@ begin
 definition llty_word :: "'a word itself \<Rightarrow> llty" where [simp]: "llty_word _ = la_i LENGTH('a)"
 definition share_word :: "zint \<Rightarrow> 'a word \<Rightarrow> 'a word" where [simp]: "share_word z = id"
 definition shareable_word :: "'a word set" where [simp]: "shareable_word = UNIV"
-definition revert_word :: "'a word \<times> 'a word \<Rightarrow> bool" where [simp]: "revert_word xy = True"
+definition revert_word :: "'a word \<Rightarrow> 'a word \<Rightarrow> bool" where [simp]: "revert_word x y = True"
 definition dpriv_word :: "'a word \<Rightarrow> 'a word" where [simp]: "dpriv_word x = x"
 definition disposable_word :: "'a word set" where [simp]: "disposable_word = UNIV"
 instance by standard auto
@@ -45,9 +45,8 @@ end
 
 instantiation word :: (len) ceq_lrep
 begin
-definition ceqable_word :: "'a word \<times> 'a word \<Rightarrow> bool" where [simp]: "ceqable_word x = True"
-definition ceq_word :: "'a word \<times> 'a word \<Rightarrow> bool" where [simp]: "ceq_word = (\<lambda>(x,y). (x = y))"
-lemma ceq_word[simp]: "ceq (x,y) = (x = y)" for x :: "'a word" by simp
+definition ceqable_word :: "'a word \<Rightarrow> 'a word \<Rightarrow> bool" where [simp]: "ceqable_word x y = True"
+definition ceq_word :: "'a word \<Rightarrow>  'a word \<Rightarrow> bool" where [simp]: "ceq_word x y = (x = y)"
 instance by standard (auto+)
 end
 
@@ -61,7 +60,7 @@ syntax "_NuNat_" :: "type \<Rightarrow> logic" (\<open>\<nat>'[_']\<close>)
 translations "\<nat>['x]" == "CONST NuNat (TYPE('x))" 
 
 lemma [simp]: "p \<nuLinkL> NuNat b \<nuLinkR> x \<equiv> (unat p = x)" unfolding NuNat_def by auto
-lemma [\<nu>intro]: "\<nu>CEqual (NuNat b) (K True) (case_prod (=))"
+lemma [\<nu>intro]: "\<nu>CEqual (NuNat b) (\<lambda>x y. True) (=)"
   unfolding \<nu>CEqual_def NuNat_def by (auto simp add: unsigned_word_eqI)
 
 definition NuNatRound :: "('a::len) itself \<Rightarrow> ('a word, nat) nu"
@@ -83,8 +82,7 @@ qed
 definition NuBool :: "(1 word, bool) nu" ("\<bool>")
   where "NuBool = Nu (\<lambda>px. case px of (p,x) \<Rightarrow> (p = 1) = x)"
 lemma [simp]: "p \<nuLinkL> \<bool> \<nuLinkR> x \<longleftrightarrow> (p = 1) = x" unfolding NuBool_def by simp
-lemma [\<nu>intro]: "\<nu>CEqual \<bool> (K True) (case_prod (=))" unfolding \<nu>CEqual_def NuBool_def by auto
-
+lemma [\<nu>intro]: "\<nu>CEqual \<bool> (\<lambda>x y. True)  (=)" unfolding \<nu>CEqual_def NuBool_def by auto
 
 
 section \<open>The pair abstract structure\<close>
@@ -97,26 +95,27 @@ instance by standard
 end
 
 instantiation prod :: (sharable_lrep, sharable_lrep) sharable_lrep begin
-definition revert_prod :: "('a \<times> 'b) \<times> ('a \<times> 'b) \<Rightarrow> bool"
-  where "revert_prod v \<longleftrightarrow> (case v of (v1,v2) \<Rightarrow> case v1 of (a1,b1) \<Rightarrow> case v2 of (a2,b2) \<Rightarrow> revert (a1,a2) \<and> revert (b1,b2))"
-lemma [simp]: "revert (v1,v2) \<longleftrightarrow> (case v1 of (a1,b1) \<Rightarrow> case v2 of (a2,b2) \<Rightarrow> revert (a1,a2) \<and> revert (b1,b2))"
+definition revert_prod :: "('a \<times> 'b) \<Rightarrow> ('a \<times> 'b) \<Rightarrow> bool"
+  where "revert_prod v1 v2 \<longleftrightarrow> (case v1 of (a1,b1) \<Rightarrow> case v2 of (a2,b2) \<Rightarrow> revert a1 a2 \<and> revert b1 b2)"
+lemma [simp]: "revert (a1,b1) (a2,b2) \<longleftrightarrow> revert a1 a2 \<and> revert b1 b2"
   unfolding revert_prod_def by simp
 definition shareable_prod :: "('a \<times> 'b) set" where "shareable_prod = shareable \<times> shareable"
 lemma [simp]: "(a,b) \<in> shareable \<longleftrightarrow> a \<in> shareable \<and> b \<in> shareable" unfolding shareable_prod_def by simp
 definition share_prod :: "zint \<Rightarrow> 'a \<times> 'b \<Rightarrow> 'a \<times> 'b" where [simp]: "share_prod z x = (case x of (a,b) \<Rightarrow> (share z a, share z b))"
 definition dpriv_prod :: "'a \<times> 'b \<Rightarrow> 'a \<times> 'b" where [simp]: "dpriv_prod x = (case x of (a,b) \<Rightarrow> (dpriv a, dpriv b))"
-instance by standard (auto, (metis revert_sym revert_trans) +)
+instance by standard (auto intro: revert_trans)
 end
 
 instantiation prod :: (naive_lrep, naive_lrep) naive_lrep
   begin instance by standard auto end
 
 instantiation prod :: (ceq_lrep, ceq_lrep) ceq_lrep begin
-definition ceqable_prod :: "('a \<times> 'b) \<times> 'a \<times> 'b \<Rightarrow> bool"
-  where [simp]: "ceqable_prod x = (case x of ((a1,b1),(a2,b2)) \<Rightarrow> ceqable (a1,a2) \<and> ceqable (b1,b2))"
-definition ceq_prod :: "('a \<times> 'b) \<times> 'a \<times> 'b \<Rightarrow> bool"
-  where [simp]: "ceq_prod x = (case x of ((a1,b1),(a2,b2)) \<Rightarrow> ceq (a1,a2) \<and> ceq (b1,b2))"
-instance by standard (auto simp add: ac_simps intro: ceq_trans)
+definition ceqable_prod :: "'a \<times> 'b \<Rightarrow> 'a \<times> 'b \<Rightarrow> bool"
+  where "ceqable_prod x y = (case x of (a1,b1) \<Rightarrow> case y of (a2,b2) \<Rightarrow> ceqable a1 a2 \<and> ceqable b1 b2)"
+lemma [simp]: "ceqable (a1,b1) (a2,b2) \<longleftrightarrow> ceqable a1 a2 \<and> ceqable b1 b2" unfolding ceqable_prod_def by auto
+definition ceq_prod :: "'a \<times> 'b \<Rightarrow> 'a \<times> 'b \<Rightarrow> bool"
+  where [simp]: "ceq_prod x y = (case x of (a1,b1) \<Rightarrow> case y of (a2,b2) \<Rightarrow> ceq a1 a2 \<and> ceq b1 b2)"
+instance by standard (auto intro: ceq_trans)
 end
 
 subsection \<open>Fusion \<nu>-abstraction\<close>
@@ -131,11 +130,55 @@ lemma "Inhabited \<tort_lbrace>(x1,x2) \<tycolon> N1 \<nuFusion> N2\<tort_rbrace
 lemma [\<nu>intro]: "\<nu>Share N s1 f1 \<Longrightarrow> \<nu>Share M s2 f2 \<Longrightarrow> \<nu>Share (N \<nuFusion> M) (s1 \<times> s2) (\<lambda>z x. case x of (x1,x2) \<Rightarrow> (f1 z x1, f2 z x2))"
   for N :: "('a :: sharable_lrep, 'b) nu" and M :: "('c :: sharable_lrep, 'd) nu" 
   unfolding \<nu>Share_def by auto
-lemma [\<nu>intro]: "\<nu>Equalable N p \<Longrightarrow> \<nu>Equalable M q \<Longrightarrow> \<nu>Equalable (N \<nuFusion> M) (\<lambda>x. case x of ((a1,b1),(a2,b2)) \<Rightarrow> p (a1,a2) \<and> q (b1,b2))"
-  unfolding \<nu>Equalable_def by auto
+lemma [\<nu>intro]: "\<nu>CEqual N p \<Longrightarrow> \<nu>CEqual M q \<Longrightarrow> \<nu>CEqual (N \<nuFusion> M) (\<lambda>x. case x of ((a1,b1),(a2,b2)) \<Rightarrow> p (a1,a2) \<and> q (b1,b2))"
+  unfolding \<nu>CEqual_def by auto
 
 lemma [\<nu>intro]: "\<nu>Disposable \<tort_lbrace>x \<tycolon> X\<tort_rbrace> \<Longrightarrow> \<nu>Disposable \<tort_lbrace>y \<tycolon> Y\<tort_rbrace> \<Longrightarrow> \<nu>Disposable \<tort_lbrace>(x,y) \<tycolon> X \<nuFusion> Y\<tort_rbrace>"
   unfolding \<nu>Disposable_def by auto
 
 
+section \<open>Tuple\<close>
+
+class field = lrep
+class field_list = lrep
+
+instantiation void :: field_list begin instance by standard end
+instantiation prod :: (field, field_list) field_list begin instance by standard end
+instantiation word :: (len) field begin instance by standard end
+
+datatype 'a tuple = Tuple "('a::field_list)"
+
+subsection \<open>Lrep instantiations\<close>
+
+instantiation tuple :: (field_list) lrep begin
+definition llty_tuple :: " 'a tuple itself \<Rightarrow> llty " where [simp]: "llty_tuple _ = la_tup (llty TYPE('a))"
+definition disposable_tuple :: " 'a tuple set " where [simp]: "disposable_tuple = image Tuple disposable"
+instance by standard
+end
+
+instantiation tuple :: ("{zero_lrep,field_list}") zero_lrep begin
+definition lty_zero_tuple :: " 'a tuple " where [simp]: "lty_zero_tuple = Tuple lty_zero"
+instance by standard
+end
+
+instantiation tuple :: ("{sharable_lrep,field_list}") sharable_lrep begin
+definition shareable_tuple :: " 'a tuple set " where [simp]: "shareable_tuple = image Tuple shareable"
+definition share_tuple :: " zint \<Rightarrow> 'a tuple \<Rightarrow> 'a tuple " where [simp]: "share_tuple z = map_tuple (share z)"
+definition revert_tuple :: " 'a tuple \<Rightarrow> 'a tuple \<Rightarrow> bool " where "revert_tuple x y = (case x of Tuple a \<Rightarrow> case y of Tuple b \<Rightarrow> revert a b)"
+lemma [simp]: "revert (Tuple a) (Tuple b) \<longleftrightarrow> revert a b" unfolding revert_tuple_def by simp
+definition dpriv_tuple :: " 'a tuple \<Rightarrow> 'a tuple " where "dpriv_tuple = map_tuple dpriv"
+instance proof
+  fix x y z :: " 'a tuple"  and a b :: zint
+  show "revert x x" by (cases x) auto
+  show "revert x y = revert y x" by (cases x, cases y) (auto simp add: revert_sym)
+  show "revert x y \<Longrightarrow> revert y z \<Longrightarrow> revert x z" by (cases x, cases y, cases z) (auto intro: revert_trans)
+  show "share (Gi 0) x = x" by (cases x) auto
+  show "share b (share a x) = share (a + b) x" by (cases x) auto
+qed
+end
+
+term "(O)"
+instantiation tuple :: ("{ceq_lrep,field_list}") ceq_lrep begin
+
+end
 end
